concurrency/Modular/templates/list_inst.v
@@ -13,27 +13,32 @@ Definition Vprog : varspecs.  mk_varspecs prog. Defined.
 
 (* struct node {int key; void *value; struct tree_t *left, *right;} node;*)
 Definition t_struct_list := Tstruct _node noattr.
+(* Define for dynamic list *)
+Definition struct_dlist := Tstruct _DList noattr.
 
-(* struct tree_t {node *t; lock_t *lock; int min; int max; } tree_t; *)
-Definition t_struct_list_t := Tstruct _list_t noattr.
-
+#[local] Obligation Tactic := idtac.
 (* node_rep_R r.1.1.1 r.1.2 r.2 g, and r is type of node_info *)
-#[local]Instance my_specific_tree_rep : NodeRep := {
-    node_rep_R :=
-      fun tp r g_info g =>
+#[local] Program Instance my_specific_tree_rep : NodeRep := {
+    node_rep_R := fun (tp : val) (r : range) (g_info : option (option ghost_info)) g =>
       if eq_dec tp nullval
       then !!(g_info = Some None) && seplog.emp
-      else (
-    EX (gn : gname), EX (x : Z), EX (v next : val), EX (lockn : val),
-      !!(g_info = Some (Some (x, v, [gn])) /\ and (Z.le Int.min_signed x) (Z.le x Int.max_signed) /\
-       is_pointer_or_null next /\ is_pointer_or_null lockn /\
-          (tc_val (tptr Tvoid) v) /\ key_in_range x r = true) &&
+      else (EX (x : Z), EX (v next : val),
+      !!(g_info = Some (Some (x, v, [next])) /\ and (Z.le Int.min_signed x) (Z.le x Int.max_signed) /\
+       is_pointer_or_null next /\ (tc_val (tptr Tvoid) v) /\ key_in_range x r = true) &&
        data_at Ews t_struct_list ((Vint (Int.repr x)), (v, next)) tp *
-       malloc_token Ews t_struct_list tp *
-       in_tree g gn next lockn)
-}.
+       malloc_token Ews t_struct_list tp); node_size := 1 }.
+Next Obligation.
+  simpl.
+  intros tp r g_info g.
+  destruct (EqDec_val tp nullval); [ | Intros x v next]; entailer !.
+Defined.
+Next Obligation.
+  simpl.
+  intros tp r g_info g.
+  destruct (EqDec_val tp nullval); [ | Intros x v next]; entailer !.
+Defined.
 
-Definition extract_node_gname (node: node_info) : list gname :=
+Definition extract_node_pn (node: node_info) : list val :=
   match node.2 with
   | Some (Some (_, _, lst)) => lst
   | _ => []
@@ -42,110 +47,154 @@ Definition extract_node_gname (node: node_info) : list gname :=
 (* Spec of findnext function *)
 (* FOUND = 0, NOTFOUND = 1, NULLNEXT = 2 (NULLNEXT = NULL || NEXT ) *)
 
+(* Spec of findnext function *)
+(* FOUND = 0, NOTFOUND = 1, NULLNEXT = 2 (NULLNEXT = NULL || NEXT ) *)
 Definition findnext_spec :=
   DECLARE _findNext
-  WITH x: Z, p: val, n: val, n_pt : val, tp: val, r : node_info, g: gname, sh: share, gv: globals
-  PRE [ tptr tvoid, tptr (tptr tvoid), tint ]
-          PROP (writable_share sh)
+  WITH x: Z, p: val, n: val, n_pt : val, r: node_info,
+                g: gname, sh: share, gv: globals
+  PRE [ tptr t_struct_list, tptr (tptr tvoid), tint ]
+          PROP (writable_share sh(*; is_pointer_or_null pa; is_pointer_or_null pb*) )
           PARAMS (p; n; Vint (Int.repr x)) GLOBALS (gv)
-          SEP (node_rep_R r.1.1.1 r.1.2 r.2 g ;
-               field_at sh (t_struct_list_t) [StructField _t] r.1.1.1 p;
-               data_at sh (tptr t_struct_list_t) n_pt n)
+          SEP (node_rep_R r.1.1.1 r.1.2 r.2 g * (!!(p = r.1.1.1 /\ p <> nullval) && seplog.emp) *
+               (* field_at sh (t_struct_tree) [StructField _t] r.1.1.1 p; *)
+               data_at sh (tptr tvoid) n_pt n)
   POST [ tint ]
-  EX (stt: enum), EX (n' next : val) (g_in : gname),
+  EX (stt: enum), EX (n' next : val),
          PROP (match stt with
                | F | NF => (n' = p)
                | NN => (n' = next)
                end)
         LOCAL (temp ret_temp (enums stt))
-        SEP (!!(g_in ∈ extract_node_gname r) &&
-               node_rep_R r.1.1.1 r.1.2 r.2 g *
-               field_at sh (t_struct_list_t) [StructField _t] r.1.1.1 p *
-               data_at sh (tptr t_struct_list_t) next n).
+        SEP (match stt with
+               | F | NF => data_at sh (tptr tvoid) n_pt n
+               | NN => !!(n' ∈ extract_node_pn r) && data_at sh (tptr tvoid) next n
+             end *
+               node_rep_R r.1.1.1 r.1.2 r.2 g) .
 
 
 Lemma findNext: semax_body Vprog Gprog f_findNext findnext_spec.
 Proof.
   start_function.
-  (* int y = pn->p->t->key *)
-  forward. 
   unfold node_rep_R.
-  destruct (eq_dec r.1.1.1 nullval).
-  + rewrite e.
-    unfold my_specific_tree_rep.
-    rewrite -> if_true; auto.
-    forward.
-    forward.
-    forward.
-  Intros gn x0 v0 next lockn.
+  unfold my_specific_tree_rep.
+  Intros.
+  subst.
+  rewrite -> if_false; eauto.
+  Intros x0 v0 next.
   forward.
-  forward.
-  forward.
-  forward_if. (* if (_x < _y) *)
-  - (* pn->n = pn->p->t->left *)
-    forward. (* t1 = pn->p *)
-    forward. (* t2 = t1->t *)
-    forward. (* t3 = t2->left *)
+  forward_if. 
+  - forward.
+    forward.
     forward.
     Exists NN.
-    Exists next next gn.
+    Exists next next.
     entailer !.
-    unfold extract_node_gname.
+    unfold extract_node_pn.
     rewrite H.
     apply elem_of_list_here.
-    Exists gn x0 v0 next lockn.
+    unfold node_rep_R.
+    simpl.
+    rewrite -> if_false; eauto.
+    Exists x0 v0 next.
     entailer !.
   - forward_if.
-    (* pn->n = pn->p->t->right *)
     repeat forward.
-    Exists NF p n_pt gn. 
+    Exists NF r.1.1.1 n_pt.
     entailer !.
-    unfold extract_node_gname.
-    rewrite H.
-    apply elem_of_list_here.
-    Exists gn x0 v0 next lockn.
+    unfold node_rep_R.
+    simpl.
+    rewrite -> if_false; eauto.
+    Exists x0 v0 next.
     entailer !.
     forward.
-    Exists F p n_pt gn.
+    Exists F r.1.1.1 n_pt.
     entailer !.
-    unfold extract_node_gname.
-    rewrite H.
-    apply elem_of_list_here.
-    Exists gn x0 v0 next lockn.
+    unfold node_rep_R.
+    simpl.
+    rewrite -> if_false; eauto.
+    Exists x0 v0 next.
     entailer !.
 Qed.
 
+Definition surely_malloc_spec :=
+  DECLARE _surely_malloc
+   WITH t: type, gv: globals
+   PRE [ size_t ]
+       PROP (and (Z.le 0 (sizeof t)) (Z.lt (sizeof t) Int.max_unsigned);
+                complete_legal_cosu_type t = true;
+                natural_aligned natural_alignment t = true)
+       PARAMS (Vptrofs (Ptrofs.repr (sizeof t))) GLOBALS (gv)
+       SEP (mem_mgr gv)
+    POST [ tptr tvoid ]
+    EX p: _,
+       PROP ()
+       RETURN (p)
+       SEP (mem_mgr gv; malloc_token Ews t p * data_at_ Ews t p).
 
-(*
-#[export] Instance pointer_lock : Ghost := discrete_PCM (val * val * range).
-Definition ghost_info : Type := (key * val)%type.
+Definition insertOp_spec :=
+  DECLARE _insertOp
+    WITH x: Z, stt: Z, v: val, p: val, tp: val, l: val, dl: val, next: list val, r: node_info,
+                    g: gname, gv: globals
+  PRE [ tptr (tptr t_struct_list), tint, tptr tvoid, tint, tptr (struct_dlist)]
+  PROP (repable_signed x; is_pointer_or_null v; key_in_range x r.1.2 = true;
+        is_pointer_or_null (Znth 0 next);
+        length next = node_size)
+  PARAMS (p; Vint (Int.repr x); v; Vint (Int.repr stt); l)
+  GLOBALS (gv)
+  SEP (mem_mgr gv; node_rep_R nullval r.1.2 r.2 g *
+                     field_at Ews (struct_dlist) [StructField _list] dl l *
+                     (* field_at Ews (struct_dlist) [StructField _size] (Vptrofs (Ptrofs.repr 2%Z)) l * *)
+                     data_at Ews (tarray (tptr tvoid) (Zlength next)) next dl * 
+                     (* (!!(p = r.1.1.1 /\ p = nullval)  && seplog.emp); *)
+       data_at Ews (tptr t_struct_list) tp p)
+  POST[ tvoid ]
+  EX (pnt : val),
+  PROP (pnt <> nullval)
+  LOCAL ()
+  SEP (mem_mgr gv; data_at Ews (tptr t_struct_list) pnt p;
+       node_rep_R pnt r.1.2 (Some (Some (x, v, next))) g;
+       field_at Ews struct_dlist (DOT _list) dl l;
+       data_at Ews (tarray (tptr tvoid) (Zlength next)) next dl).
 
-(* This allows the range to be outdated while the ghost_info may be present or absent. *)
-#[export] Instance node_ghost : Ghost := prod_PCM pointer_lock (exclusive_PCM (option ghost_info)).
-Notation node_info := (@G node_ghost).
+Lemma length_equal_1 : forall (x: Z) (v: val) (next : list val),
+  length next = 1%nat ->
+  Some (Some (x, v, next)) = Some (Some (x, v, [Znth 0 next])).
+Proof.
+  intros x v next H_length.
+  destruct next as [|a [|b tl]] eqn:Heq_next; try discriminate.
+  inversion H_length; subst.
+  unfold Znth; simpl.
+  repeat f_equal.  
+Qed.
 
-Definition in_tree (g: gname) (g1 : gname) (pn: val) (lock: val):=
-      ghost_snap (P := gmap_ghost (K := gname)(A := discrete_PCM (val * val)) )
-        ({[g1 := (pn, lock)]}) g.
-
-Lemma in_tree_duplicate g gin pn lock:
-  in_tree g gin pn lock |-- in_tree g gin pn lock * in_tree g gin pn lock.
-Proof. by rewrite - bi.persistent_sep_dup. Qed.
-
-Class NodeRep : Type := {
-  node_rep_R : val -> range -> option (option ghost_info) -> gname -> mpred
-  }.
-
-
-#[export]Instance my_specific_tree_rep : NodeRep := {
-  node_rep_R := fun tp r g_info g =>
-    EX (ga gb : gname), EX (x : Z), EX (v pa pb : val), EX (locka lockb : val),
-      !!(g_info = Some (Some (x, v)) /\ and (Z.le Int.min_signed x) (Z.le x Int.max_signed) /\
-       is_pointer_or_null pa /\ is_pointer_or_null locka /\
-       is_pointer_or_null pb /\ is_pointer_or_null lockb /\
-          (tc_val (tptr Tvoid) v) /\ key_in_range x r = true) &&
-       data_at Ews t_struct_tree ((Vint (Int.repr x)), (v, (pa, pb))) tp * 
-       malloc_token Ews t_struct_tree tp *
-       in_tree g ga pa locka * in_tree g gb pb lockb
-}.
-*)
+Definition Gprog : funspecs :=
+    ltac:(with_library prog [acquire_spec; release_spec; makelock_spec;
+     surely_malloc_spec; insertOp_spec (* ; traverse_spec; insert_spec; treebox_new_spec*) ]).
+(* Proving insertOp satisfies spec *)
+Lemma insertOp: semax_body Vprog Gprog f_insertOp insertOp_spec.
+Proof.
+  start_function.
+  forward_call (t_struct_list, gv).
+  Intros new_node.
+  forward.
+  forward.
+  forward.
+  forward.
+  entailer !.
+  simpl in H3.
+  rewrite Zlength_correct. lia.
+  forward.
+  forward.
+  Exists new_node.
+  assert_PROP (new_node <> nullval). entailer !.
+  unfold node_rep_R.
+  unfold my_specific_tree_rep.
+  rewrite if_false; auto.
+  destruct (eq_dec nullval nullval); last first; try easy.
+  Intros.
+  entailer !.
+  Exists x v.
+  Exists (Znth 0 next).
+  entailer !. by apply length_equal_1.
+Qed.
